src/Std/Tactic/BVDecide/Normalize/BitVec.lean
@@ -57,8 +57,8 @@ theorem BitVec.sle_eq_ult (x y : BitVec w) :
 attribute [bv_normalize] BitVec.ofNat_eq_ofNat
 
 @[bv_normalize]
-theorem BitVec.ofNatLt_reduce (n : Nat) (h) : BitVec.ofNatLt n h = BitVec.ofNat w n := by
-  simp [BitVec.ofNatLt, BitVec.ofNat, Fin.ofNat', Nat.mod_eq_of_lt h]
+theorem BitVec.ofNatLT_reduce (n : Nat) (h) : BitVec.ofNatLT n h = BitVec.ofNat w n := by
+  simp [BitVec.ofNatLT, BitVec.ofNat, Fin.ofNat', Nat.mod_eq_of_lt h]
 
 @[bv_normalize]
 theorem BitVec.ofBool_eq_if (b : Bool) : BitVec.ofBool b = bif b then 1#1 else 0#1 := by
